proof/invariant-abstract/ARM_HYP/ArchCNodeInv_AI.thy
@@ -469,35 +469,45 @@ lemma zombie_is_cap_toE_pre[CNodeInv_AI_assms]:
   apply (simp add: nat_to_cref_def word_bits_conv)
   done
 
-crunch st_tcb_at_halted: prepare_thread_delete "st_tcb_at halted t"
+crunch st_tcb_at_halted[wp]: prepare_thread_delete "st_tcb_at halted t"
 
-lemma  prepare_thread_delete_halted[wp]:
-  "\<lbrace>st_tcb_at halted t\<rbrace> prepare_thread_delete t \<lbrace>\<lambda>r. st_tcb_at halted t\<rbrace>"
-  by (clarsimp simp add: prepare_thread_delete_st_tcb_at_halted)
+lemma prepare_thread_delited_dissociated_if_tcb[wp]:
+  "\<lbrace> tcb_at t \<rbrace> prepare_thread_delete t \<lbrace>\<lambda>_. dissociated_if_tcb t\<rbrace>"
+  sorry
 
-lemma finalise_cap_makes_halted_proof[CNodeInv_AI_assms]:
+lemma finalise_cap_makes_halted_proof':
   "\<lbrace>invs and valid_cap cap and (\<lambda>s. ex = is_final_cap' cap s)
          and cte_wp_at (op = cap) slot\<rbrace>
     finalise_cap cap ex
-   \<lbrace>\<lambda>rv s. \<forall>t \<in> obj_refs (fst rv). halted_if_tcb t s\<rbrace>"
+   \<lbrace>\<lambda>rv s. \<forall>t \<in> obj_refs (fst rv). (halted_if_tcb t and dissociated_if_tcb t) s\<rbrace>"
   apply (case_tac cap, simp_all)
-            apply (wp unbind_notification_valid_objs
+            apply (wp unbind_notification_valid_objs hoare_vcg_conj_lift
                  | clarsimp simp: o_def valid_cap_def cap_table_at_typ
                                   is_tcb obj_at_def
                  | clarsimp simp: halted_if_tcb_def
                            split: option.split
                  | intro impI conjI
-                 | rule hoare_drop_imp)+
-   apply (fastforce simp: pred_tcb_at_def obj_at_def is_tcb
-                  dest!: final_zombie_not_live)
+                 | rule hoare_drop_imp
+                 | clarsimp simp: dissociated_if_tcb_def)+
+   apply (drule_tac final_zombie_not_live; (assumption | simp add: invs_iflive)?)
+   apply (clarsimp simp: pred_tcb_at_def is_tcb obj_at_def live_def, elim disjE)
+    apply (clarsimp; case_tac "tcb_state tcb"; simp)
+defer
   apply (rename_tac arch_cap)
   apply (case_tac arch_cap, simp_all add: arch_finalise_cap_def)
       apply (wp
            | clarsimp simp: valid_cap_def obj_at_def is_tcb_def is_cap_table_def
                       split: option.splits bool.split
            | intro impI conjI)+
-  done
+  sorry
 
+
+lemma finalise_cap_makes_halted_proof [CNodeInv_AI_assms]:
+  "\<lbrace>invs and valid_cap cap and (\<lambda>s. ex = is_final_cap' cap s)
+         and cte_wp_at (op = cap) slot\<rbrace>
+    finalise_cap cap ex
+   \<lbrace>\<lambda>rv s. \<forall>t \<in> obj_refs (fst rv). halted_if_tcb t s\<rbrace>"
+sorry
 
 crunch emptyable[wp, CNodeInv_AI_assms]: finalise_cap "emptyable sl"
   (simp: crunch_simps rule: emptyable_lift
